example2.v
@@ -1,0 +1,193 @@
+Require Import Autosubst.Autosubst.
+Require Import Zee.lattice Zee.lang Zee.dec Zee.vals Zee.frame Zee.maplike Zee.sem Zee.typesystem.
+Require Import Arith List Coq.Program.Basics Coq.Lists.ListSet Lia Coq.ZArith.BinInt.
+Require Import Coq.Classes.RelationClasses.
+
+Section Example2.
+  Context {A : Set} {BinOpS : Set} `{lattice A}.
+  Context {MINUS MULT : BinOpS}.
+  Definition Lab := @Lab A.
+  Definition Ty := @Ty A.
+  Definition LabVar := @LabVar A.
+  Definition SecTy := @SecTy A.
+  Definition SecTyV := @SecTyV A.
+  Definition AtomSecTy := @AtomSecTy A.
+  Definition Cmd := @Cmd A BinOpS.
+  Definition Expr := @Expr A BinOpS.
+  Definition V := @V A.
+
+  Context {δ : string -> option Z}.
+  Context {F: string -> option (list (string * Lab) *
+                               list (string * Lab) *
+                               list (string * SecTy) * Lab * Lab * Cmd) }.
+  Context {eval_binop: BinOpS -> V -> V -> V}.
+  Context {type_binop: BinOpS -> SecTy -> SecTy -> SecTy -> Prop}.
+  Context {VarT ArgT LocT MemT : Type}
+          {H_var_finmaplike: FinMapLike VarT string (A + SecTyV)}
+          {H_arg_finmaplike: FinMapLike ArgT string SecTyV}
+          {H_loc_finmaplike: FinMapLike LocT string SecTyV}
+          {H_mem_maplike: MapLike MemT nat V}.
+  Definition Frame := @Frame A VarT ArgT LocT MemT _ _ _ _.
+  Definition PFrame := @PFrame A VarT ArgT LocT _ _ _.
+  Definition EFrame := @EFrame A MemT _.
+
+  Notation "o ':' s1 ',' s2 '⤇' s" := (type_binop o s1 s2 s) (at level 70, s at next level).
+ 
+  Definition Var := @Var A BinOpS.
+  Definition Num := @Num A BinOpS.
+  Hint Unfold Var Num.
+  Coercion Var: string >-> lang.Expr.
+  Coercion Num: nat >-> lang.Expr.
+  Coercion STy: lang.Ty >-> Funclass.
+  Coercion eval_binop : BinOpS >-> Funclass.
+  
+  Definition public_varty (x : string) := VarTy x ⊥.
+  Coercion public_varty: string >-> lang.AtomSecTy.
+
+  Coercion SPat : lang.Pat >-> Funclass.
+  Coercion PVar: string >-> AtomPat.
+  
+  Definition program : Cmd :=
+    UNPACKTY "α" AS TYPE ⊥, "x" AS "α" ::=
+      TYPACK (IntTy ⊥, 42)
+        AS ∃ ("α" ::: ⊥) "α" IN
+      LET "y" AS (IntTy ⊥) ::= 0 IN
+        MATCH "α" WITH
+          (PProd "β" "γ", SKIP)
+        | (PAtom (PInt "κ"), &("y") *= Num 1)
+        ENDMATCH
+      ENDLET
+    ENDUNPACKTY.
+  Hint Unfold program.
+
+  Definition step_many := @step_many A BinOpS _ δ F eval_binop _ _ _ _ _ _ _ _.
+  Notation "cfg1 '-->[' n ']' cfg2" := (step_many cfg1 cfg2 n) (at level 80).
+  Notation "cfg1 '-->*' cfg2" := (exists n, cfg1 -->[n] cfg2) (at level 80).
+
+  Definition wt := @wt A BinOpS _ F type_binop.
+  Notation "'[' Γ ',' Π ',' ϕ ',' pc ',' fr ']' '⊢' c" := (wt Γ Π ϕ pc fr c) (at level 70, c at next level).
+
+  Lemma program_is_wt:
+    [∅, ∅, nil, ⊥, ⊥] ⊢ program.
+  Proof.
+    unfold program.
+    eapply WtUnpTy.
+    - eapply wt_packty.
+      + eapply eq_rewrite4_Proper.
+        * eapply MorphismUR_wt_sectype.
+        * rewrite <- idem_join.
+          reflexivity.
+        * do 2 constructor; constructor.
+      + do 2 constructor.
+        * reflexivity.
+        * constructor.
+      + eapply wt_sub.
+        * constructor.
+        * cbn.
+          eapply sub_atom.
+          constructor.
+          unfold flowsto_with.
+          intros.
+          reflexivity.
+    - do 2 constructor.
+      rewrite -> idem_join.
+      reflexivity.
+    - constructor.
+      constructor.
+      + reflexivity.
+      + constructor.
+    - eapply WtLet.
+      + constructor.
+      + do 2 constructor; constructor.
+      + do 2 constructor.
+        rewrite -> idem_join.
+        reflexivity.
+      + repeat rewrite -> idem_join.
+        reflexivity.
+      + eapply WtMatch.
+        * reflexivity.
+        * reflexivity.
+        * intros.
+          destruct i.
+          {
+            cbn in H.
+            inversion H; subst; clear H.
+            rewrite -> subst_secty_cmd_skip.
+            constructor.
+          }
+          {
+            destruct i.
+            - cbn in H.
+              inversion H; subst; clear H.
+              rewrite -> subst_secty_cmd_write.
+              rewrite -> subst_secty_expr_addrof.
+              unfold Num.
+              rewrite -> subst_secty_expr_num.
+              eapply WtWrite.
+              + constructor.
+                reflexivity.
+              + constructor.
+              + cbn.
+                constructor.
+                constructor.
+                unfold flowsto_with.
+                intros.
+                intro.
+                cbn.
+                rewrite -> join_bot.
+                eapply idem_join.
+            - cbn in H.
+              eapply nth_error_In in H.
+              firstorder.
+          }
+  Qed.
+          
+  Goal
+    exists stk q,
+      δ "x" = Some 0%Z ->
+      δ "y" = Some 1%Z ->
+      ⟨program, initial_stk program, 0, 0⟩ -->* ⟨CStop, stk, q, 0⟩ /\
+      stk ? 1 + fp_of (initial_stk program) = Some (VNum 1).
+  Proof.
+    do 2 eexists.
+    intros.
+    split.
+    {
+      eexists.
+      unfold program.
+      eapply StepManyS.
+      - constructor.
+        + constructor.
+          * constructor; repeat constructor.
+          * constructor.
+        + simpl.
+          constructor. constructor.
+          * simpl.
+            solve_mapsto.
+          * constructor.
+        + eassumption.
+      - cbn. eapply StepManyS.
+        + step_seq.
+          step_let.
+          intro; discriminate.
+        + cbn.
+          eapply StepManyS.
+          * repeat step_seq; try discriminate.
+            -- step_match.
+            -- intro; discriminate.
+          * cbn. eapply StepManyS.
+            repeat step_seq; try discriminate.
+            -- cbn.
+               step_write.
+            -- eapply StepManyS.
+               step_seq.
+               constructor.
+               cbn. eapply StepManyS. constructor. eapply StepMany0.
+    }
+    {
+      simpl_mapsto.
+      reflexivity.
+    }
+  Qed.
+
+End Example2.
